add example for reasoning about function with local vars

interp_test/add.v
@@ -19,13 +19,14 @@ Require Import ExtLib.Structures.Monad.
 From MetaCoq.Template Require Import bytestring MCString.
 From Coq Require Import ZArith List.
 
-From CertiCoq Require Import LambdaANF.cps LambdaANF.cps_show CodegenWASM.wasm_map_util.
+From CertiCoq Require Import LambdaANF.cps LambdaANF.cps_show CodegenWASM.wasm_map_util CodegenWASM.LambdaANF_to_WASM.
 Import MonadNotation.
 
 From Coq.Strings Require Import Byte.
 
-From Wasm Require Import binary_format_parser binary_format_printer
+From Wasm Require Import binary_format_parser binary_format_printer host
                          datatypes_properties check_toks instantiation.
+
 
 
 Module TestModule.
@@ -34,6 +35,33 @@ Definition test_bytes : list Byte.byte := x00 :: x61 :: x73 :: x6d :: x01 :: x00
 
 Definition test_module_opt : option module := run_parse_module test_bytes.
 Compute test_module_opt.
+
+From mathcomp Require Import seq.
+
+Definition test_module := {|
+  mod_types := [:: Tf [:: T_i32; T_i32] [:: T_i32]];
+  mod_funcs :=
+    [:: {|
+          modfunc_type := Mk_typeidx 0;
+          modfunc_locals := [::];
+          modfunc_body :=
+            [:: BI_get_local 0; BI_get_local 1;
+                BI_binop T_i32 (Binop_i BOI_add)]
+        |}];
+  mod_tables := [::];
+  mod_mems := [::];
+  mod_globals := [::];
+  mod_elem := [::];
+  mod_data := [::];
+  mod_start := None;
+  mod_imports := [::];
+  mod_exports :=
+    [:: {|
+          modexp_name := [:: "a"; "d"; "d"; "_"; "i"; "3"; "2"];
+          modexp_desc := MED_func (Mk_funcidx 0)
+        |}]
+|}.
+
 
 Definition type_check_test_module :=
   m <- test_module_opt ;;
@@ -44,7 +72,7 @@ Compute type_check_test_module.
 Definition test_function_type := Tf [T_i32; T_i32] [T_i32].
 Definition test_function := {|
                 modfunc_type := Mk_typeidx 0;
-                modfunc_locals := [];
+                modfunc_locals := [T_i32];
                 modfunc_body :=
                   [BI_get_local 0; BI_get_local 1;
                   BI_binop T_i32 (Binop_i BOI_add)]
@@ -61,30 +89,535 @@ From mathcomp Require Import eqtype.
 From Wasm Require Import host opsem instantiation.
 
 Section OpsemTest.
-Variable host_function : eqType.
-Let host := host host_function.
-
-Variable host_instance : host.
-
-Let store_record := store_record host_function.
-Let host_state := host_state host_instance.
-
 Require Import Lia.
 Import Relations.Relation_Operators.
 
+From Wasm Require Import interpreter_sound.
+
+From mathcomp Require Import ssreflect ssrfun ssrnat ssrbool eqtype seq.
+From StrongInduction Require Import StrongInduction Inductions.
+
+Set Implicit Arguments.
+Unset Strict Implicit.
+Unset Printing Implicit Defensive.
+
+
+From Wasm Require Import operations opsem interpreter_func interpreter_func_sound properties common.
+
+Variable host_function : eqType.
+Let store_record := store_record host_function.
+Let function_closure := function_closure host_function.
+(*Let administrative_instruction := administrative_instruction host_function.
+
+Let to_e_list : seq basic_instruction -> seq administrative_instruction := @to_e_list _.
+Let to_b_list : seq administrative_instruction -> seq basic_instruction := @to_b_list _.*)
+Let e_typing : store_record -> t_context -> seq administrative_instruction -> function_type -> Prop :=
+  @e_typing _.
+Let inst_typing : store_record -> instance -> t_context -> bool := @inst_typing _.
+(*Let reduce_simple : seq administrative_instruction -> seq administrative_instruction -> Prop :=
+  @reduce_simple _.
+Let const_list : seq administrative_instruction -> bool := @const_list _.
+Let lholed := lholed host_function.
+Let lfilled : depth -> lholed -> seq administrative_instruction -> seq administrative_instruction -> bool :=
+  @lfilled _.
+Let lfilledInd : depth -> lholed -> seq administrative_instruction -> seq administrative_instruction -> Prop :=
+  @lfilledInd _.
+Let es_is_basic : seq administrative_instruction -> Prop := @es_is_basic _.*)
+
+Let host := host host_function.
+
+(*Let run_one_step_fuel := @run_one_step_fuel host_function.*)
+
+Let RS_crash := interpreter_func.RS_crash.
+Let RS_break := interpreter_func.RS_break.
+Let RS_return := interpreter_func.RS_return.
+Let RS_normal := interpreter_func.RS_normal.
+
+Variable host_instance : host.
+
+Let run_step_fuel := @run_step_fuel host_function host_instance.
+
+Let host_state := host_state host_instance.
+
+Let reduce : host_state -> store_record -> frame -> seq administrative_instruction ->
+             host_state -> store_record -> frame -> seq administrative_instruction -> Prop
+  := @reduce _ _.
+
+Variable host_application_impl : host_state -> store_record -> function_type -> host_function -> seq value ->
+                       (host_state * option (store_record * result)).
+
+Hypothesis host_application_impl_correct :
+  (forall hs s ft hf vs hs' hres, (host_application_impl hs s ft hf vs = (hs', hres)) -> host_application hs s ft hf vs hs' hres).
+
+Let run_one_step := @run_one_step host_function host_instance host_application_impl.
+Let run_step := @run_step host_function host_instance host_application_impl.
+Let run_step_with_fuel := @run_step_with_fuel host_function host_instance host_application_impl.
+
+(** The lemmas [r_eliml] and [r_elimr] are the fundamental framing lemmas.
+  They enable to focus on parts of the stack, ignoring the context. **)
+
+Lemma r_eliml: forall s f es s' f' es' lconst hs hs',
+    const_list lconst ->
+    reduce hs s f es hs' s' f' es' ->
+    reduce hs s f (lconst ++ es) hs' s' f' (lconst ++ es').
+Proof.
+  move => s f es s' f' es' lconst hs hs' HConst H.
+  apply: r_label; try apply/lfilledP.
+  - by apply: H.
+  - replace (lconst++es) with (lconst++es++[::]); first by apply: LfilledBase.
+    f_equal. by apply: cats0.
+  - replace (lconst++es') with (lconst++es'++[::]); first by apply: LfilledBase.
+    f_equal. by apply: cats0.
+Qed.
+
+Lemma r_elimr: forall s f es s' f' es' les hs hs',
+    reduce hs s f es hs' s' f' es' ->
+    reduce hs s f (es ++ les) hs' s' f' (es' ++ les).
+Proof.
+  move => s f es s' f' es' les hs hs' H.
+  apply: r_label; try apply/lfilledP.
+  - apply: H.
+  - replace (es++les) with ([::]++es++les) => //. by apply: LfilledBase.
+  - replace (es'++les) with ([::]++es'++les) => //. by apply: LfilledBase.
+Qed.
+
+(** [r_eliml_empty] and [r_elimr_empty] are useful instantiations on empty stacks. **)
+
+Lemma r_eliml_empty: forall s f es s' f' lconst hs hs',
+    const_list lconst ->
+    reduce hs s f es hs' s' f' [::] ->
+    reduce hs s f (lconst ++ es) hs' s' f' lconst.
+Proof.
+  move => s f es s' f' lconst hs hs' HConst H.
+  assert (reduce hs s f (lconst++es) hs' s' f' (lconst++[::])); first by apply: r_eliml.
+  by rewrite cats0 in H0.
+Qed.
+
+Lemma r_elimr_empty: forall s f es s' f' les hs hs',
+    reduce hs s f es hs' s' f' [::] ->
+    reduce hs s f (es ++ les) hs' s' f' les.
+Proof.
+  move => s f es s' f' les hs hs' H.
+  assert (reduce hs s f (es++les) hs' s' f' ([::] ++les)); first by apply: r_elimr.
+  by rewrite cat0s in H0.
+Qed.
+
+Lemma run_step_fuel_not_zero : forall tt,
+  run_step_fuel tt <> 0.
+Proof.
+  move=> [[st vs] es].
+  rewrite/run_step_fuel.
+  unfold interpreter_func.run_step_fuel.
+  destruct st.
+  by lias.
+Qed.
+
+Local Lemma ves_projection: forall vs e es vs' e' es',
+  const_list vs ->
+  const_list vs' ->
+  ~ is_const e ->
+  ~ is_const e' ->
+  vs ++ e :: es = vs' ++ e' :: es' ->
+  e = e'.
+Proof.
+  move => vs. induction vs => //=.
+  - move => e es vs' e' es' _ HConstList HNConst HNConst'.
+    destruct vs' => //=.
+    + move => H. by inversion H.
+    + simpl in HConstList. move => H. inversion H. subst.
+      move/andP in HConstList. destruct HConstList as [Ha _].
+      rewrite Ha in HNConst. exfalso. by apply HNConst.
+  - move => e es vs' e' es' HConstList HConstList' HNConst HNConst'.
+    destruct vs' => //=.
+    + move => H. inversion H. subst.
+      move/andP in HConstList. destruct HConstList as [He' _].
+      exfalso. by apply HNConst'.
+    + simpl in HConstList'. move => H. inversion H. subst.
+      move/andP in HConstList. move/andP in HConstList'.
+      destruct HConstList as [Ha Hvs]. destruct HConstList' as [Ha' Hvs'].
+      eapply IHvs => //=.
+      * by apply Hvs'.
+      * by apply H2.
+Qed.
+
+Lemma lfilled0: forall es,
+  lfilledInd 0 (LH_base [::] [::]) es es.
+Proof.
+  move => es.
+  assert (lfilledInd 0 (LH_base [::] [::]) es ([::]++es++[::])) as H; first by apply LfilledBase.
+  simpl in H. by rewrite cats0 in H.
+Qed.
+
+Lemma lfilled0_frame_l: forall vs es es' LI vs',
+  lfilledInd 0 (LH_base vs es') es LI ->
+  const_list vs' ->
+  lfilledInd 0 (LH_base (vs' ++ vs) es') es (vs' ++ LI).
+Proof.
+  move => vs es es' LI vs' HLF HConst. inversion HLF; subst; clear HLF.
+  assert (HList: vs' ++ vs ++ es ++ es' = (vs' ++ vs) ++ es ++ es'); first by repeat rewrite catA.
+  rewrite HList.
+  apply LfilledBase. by rewrite const_list_concat.
+Qed.
+
+Lemma lfilled0_frame_l_empty: forall es es' LI vs',
+  lfilledInd 0 (LH_base [::] es') es LI ->
+  const_list vs' ->
+  lfilledInd 0 (LH_base vs' es') es (vs' ++ LI).
+Proof.
+  move => es es' LI vs' HLF HConst. inversion HLF; subst; clear HLF.
+  repeat rewrite catA.
+  rewrite cats0.
+  rewrite -catA.
+  by apply LfilledBase.
+Qed.
+
+Lemma lfilled0_frame_r: forall vs es es' LI es'',
+  lfilledInd 0 (LH_base vs es') es LI ->
+  lfilledInd 0 (LH_base vs (es' ++ es'')) es (LI ++ es'').
+Proof.
+  move => vs es es' LI es'' HLF. inversion HLF; subst; clear HLF.
+  repeat rewrite -catA.
+  by apply LfilledBase.
+Qed.
+
+Lemma lfilled0_frame_r_empty: forall vs es LI es'',
+  lfilledInd 0 (LH_base vs [::]) es LI ->
+  lfilledInd 0 (LH_base vs es'') es (LI ++ es'').
+Proof.
+  move => vs es LI es'' HLF. inversion HLF; subst; clear HLF.
+  repeat rewrite -catA.
+  by apply LfilledBase.
+Qed.
+
+Lemma lfilled0_take_drop: forall vs es n es',
+  const_list vs ->
+  n <= size vs ->
+  lfilledInd 0 (LH_base (take n vs) es') (drop n vs ++ es) (vs ++ es ++ es').
+Proof.
+  move => vs es n es' HConst HSize.
+  replace (vs++es++es') with (take n vs ++ (drop n vs ++ es) ++ es').
+  apply LfilledBase. by apply const_list_take.
+  { repeat rewrite catA. by rewrite cat_take_drop. }
+Qed.
+
+(** The following tactics are meant to help the proof of [run_step_soundness] below. **)
+
+(** Simplify an hypothesis, possibly rewriting it everywhere. **)
+Ltac simplify_hypothesis Hb :=
+  repeat rewrite length_is_size in Hb;
+  repeat match type of Hb with
+  | is_true (es_is_trap _) => move/es_is_trapP: Hb => Hb
+  | is_true (const_list (_ :: _)) => rewrite const_list_cons in Hb
+  | ?b = true => fold (is_true b) in Hb
+  | (_ == _) = false => move/eqP in Hb
+  | context C [size (rev _)] => rewrite size_rev in Hb
+  | context C [take _ (rev _)] => rewrite take_rev in Hb
+  | context C [rev (rev _)] => rewrite revK in Hb
+  | context C [true && _] => rewrite Bool.andb_true_l in Hb
+  | context C [_ && true] => rewrite Bool.andb_true_r in Hb
+  | context C [false || _] => rewrite Bool.orb_false_l in Hb
+  | context C [_ || false] => rewrite Bool.orb_false_r in Hb
+  | is_true true => clear Hb
+  | is_true false => exfalso; apply: notF; apply: Hb
+  | is_true (_ == _) => move/eqP in Hb
+  | ?x = ?x => clear Hb
+  | _ = _ => rewrite Hb in *
+  end.
+
+(** Apply [simplify_hypothesis] to all hypotheses. **)
+Ltac simplify_goal :=
+  repeat match goal with H: _ |- _ => progress simplify_hypothesis H end.
+
+(** A common pattern in the proof: using an hypothesis on the form [rev l = l'] to rewrite [l]. **)
+Ltac subst_rev_const_list :=
+ repeat lazymatch goal with
+ | HRevConst: rev ?lconst = ?h :: ?t |- _ =>
+   apply rev_move in HRevConst; rewrite HRevConst; rewrite -cat1s; rewrite rev_cat;
+   rewrite -v_to_e_cat; rewrite -catA
+ end.
+
+(** Simplify the lists in the goal. **)
+Ltac simplify_lists :=
+  (** Common rewriting rules. **)
+  repeat first [
+      rewrite drop_rev
+    | rewrite take_rev
+    | rewrite revK
+    | rewrite length_is_size
+    | rewrite size_take
+    | rewrite size_drop
+    | rewrite size_rev
+    | rewrite v_to_e_size
+    | rewrite rev_cat
+    | rewrite rev_cons -cats1
+    | rewrite -v_to_e_cat
+    | rewrite -v_to_e_rev
+    | rewrite -v_to_e_take
+    | rewrite -v_to_e_drop];
+  (** Putting all the lists into a normal form, as concatenations of as many things.
+    Because [cat1s] conflicts with [cats0], replacing any occurence of [[X]] to
+    [[X] ++ [::]], it has to be done separately.
+    Rewrite with the associated [math goal with] is avoid to deal with existential
+    vairables. **)
+  repeat match goal with
+  |- context C [?x :: ?l] =>
+     lazymatch l with [::] => fail | _ => rewrite -(cat1s x l) end
+  end;
+  repeat lazymatch goal with
+  | |- context C [[::] ++ _] => rewrite cat0s
+  | |- context C [_ ++ [::]] => rewrite cats0
+  | |- context C [rcons _ _] => rewrite -cats1
+  | |- context C [(_ ++ _) ++ _] => rewrite -catA
+  | |- context C [rev [::]] => rewrite rev0
+  | |- context C [v_to_e_list [::]] => rewrite v_to_e_list0
+  | |- context C [v_to_e_list [:: _]] => rewrite v_to_e_list1
+  end;
+  try subst_rev_const_list.
+
+(** Explode a tuple into all its components. **)
+Ltac explode_value v :=
+  lazymatch type of v with
+  | (_ * _)%type =>
+    let v1 := fresh "v1" in
+    let v2 := fresh "v2" in
+    destruct v as [v1 v2];
+    explode_value v1;
+    explode_value v2
+  | _ => idtac
+  end.
+
+(** Try to find which variable to pattern match on, destruct it,
+  then simplify the destructing equality. **)
+Ltac explode_and_simplify :=
+  repeat lazymatch goal with
+  | |- ?T = _ -> _ =>
+    lazymatch T with
+    | context C [split_n ?l ?n] => rewrite (split_n_is_take_drop l n)
+    | context C [vs_to_es ?l] => rewrite/vs_to_es
+    | context C [host_application_impl _ _ _ _ _ _] =>
+      destruct host_application_impl
+    | context C [match ?b with true => ?v1 | false => ?v2 end] =>
+      let Hb := fresh "if_expr" in
+      destruct b eqn:Hb;
+      simplify_hypothesis Hb;
+      try by [|apply: Hb]
+    | context C [match rev ?lconst with
+                 | _ :: _ => _
+                 | _ => _
+                 end] =>
+      let HRevConst := fresh "HRevConst" in
+      destruct (rev lconst) eqn:HRevConst;
+      simplify_hypothesis HRevConst;
+      try by [|apply: HRevConst]
+    | context C [match ?v with
+                 | VAL_int32 _ => _
+                 | _ => _
+                 end] =>
+      let Hb := fresh "Ev" in
+      destruct v eqn:Hb;
+      simplify_hypothesis Hb;
+      try by []
+    | context C [match ?v with
+                 | Some _ => _
+                 | _ => _
+                 end] =>
+      let Hv := fresh "option_expr" in
+      let v' := fresh "v" in
+      destruct v as [v'|] eqn:Hv; [ explode_value v' |];
+      simplify_hypothesis Hv;
+      try by [|apply: Hv]
+    | context C [match ?cl with
+                 | FC_func_native _ _ _ _ => _
+                 | FC_func_host _ _ => _
+                 end] =>
+      let Hcl := fresh "Hcl" in
+      destruct cl eqn:Hcl;
+      simplify_hypothesis Hcl;
+      try by []
+    | context C [match ?tf with
+                 | Tf _ _ => _
+                 end] =>
+      let Hcl := fresh "Htf" in
+      destruct tf eqn:Htf;
+      simplify_hypothesis Htf;
+      try by []
+    | context C [match ?v with
+                 | T_i32 => _
+                 | T_i64 => _
+                 | T_f32 => _
+                 | T_f64 => _
+                 end] =>
+      let Hv := fresh "Ev" in
+      destruct v eqn:Hv;
+      simplify_hypothesis Hv;
+      try by []
+    | context C [match ?v with
+                 | CVO_convert => _
+                 | CVO_reinterpret => _
+                 end] =>
+      let Hv := fresh "Ecvtop" in
+      destruct v eqn:Hv;
+      simplify_hypothesis Hv;
+      try by []
+    | context C [match ?v with
+                 | Tf _ _ => _
+                 end] =>
+      let vs1 := fresh "vs" in
+      let vs2 := fresh "vs" in
+      let Hv := fresh "Eft" in
+      destruct v as [vs1 vs2] eqn:Hv;
+      simplify_hypothesis Hv;
+      try by []
+    | context C [expect ?X ?f ?err] =>
+       let HExpect := fresh "HExpect" in
+       destruct X eqn:HExpect;
+       simplify_hypothesis HExpect;
+       simpl;
+       try by [|apply: HExpect]
+    | context C [match ?l with
+                 | _ :: _ => _
+                 | _ => _
+                 end] =>
+      destruct l;
+      try by []
+    end
+  end;
+  simplify_lists.
+
+(** If the goal is on the form [c1 = c2 -> property] where [c1] and [c2] are two configurations,
+  then invert it. **)
+Ltac pattern_match :=
+  let go _ :=
+    lazymatch goal with
+    | |- (_, _, _, _) = (_, _, _, _) -> _ =>
+      let H := fresh in
+      move=> H; inversion H; subst; clear H
+    end in
+  go tt || (simpl; go tt).
+
+(** Eliminate the stack frame, by applying [r_elimr] and [r_eliml] according to some heuristics. **)
+Ltac stack_frame :=
+  repeat lazymatch goal with
+  | |- reduce _ _ _ (_ :: ?l) _ _ _ _ =>
+    rewrite -cat1s
+  | |- reduce _ _ _ (?l1 ++ ?l2 :: ?l3) _ _ _ ((?l5 ++ ?l4) ++ ?l3) =>
+    rewrite -cat1s; rewrite catA;
+    apply: r_elimr; try apply: r_eliml; try apply: v_to_e_is_const_list
+  | |- reduce _ _ _ (?l1 ++ ?l2 :: ?l3) _ _ _ (?l5 ++ ?l3) =>
+    rewrite -cat1s; rewrite catA;
+    apply: r_elimr; try apply: r_eliml_empty; try apply: v_to_e_is_const_list
+  | |- reduce _ _ _ (operations.v_to_e_list ?l1 ++ _) _ _ _ (operations.v_to_e_list (take ?n ?l1) ++ _) =>
+    rewrite (v_to_e_take_drop_split l1 n); rewrite -catA;
+    apply: r_eliml; try apply: v_to_e_is_const_list
+  end.
+
+(** Try to solve a goal of the form [const_list _]. **)
+Ltac solve_const_list :=
+  repeat rewrite const_list_concat;
+  repeat rewrite const_list_cons;
+  by [| apply: v_to_e_is_const_list ].
+
+(** Try to solve a goal of the form [l1 = l2] where [l1] and [l2] are two lists. **)
+Ltac show_list_equality :=
+  simplify_lists; simplify_goal;
+  by [| repeat f_equal
+      | repeat rewrite catA; repeat f_equal
+      | repeat rewrite -catA; repeat f_equal
+      | eauto
+      | erewrite cats0; eauto
+      | erewrite cat0s; eauto
+      | repeat (repeat rewrite catA; f_equal; repeat rewrite -catA; f_equal)
+      | repeat (repeat rewrite -catA; f_equal; repeat rewrite catA; f_equal) ].
+
+(** Given a left and a right frame, rewrite the goal to move these frames out. **)
+Ltac frame_out l r :=
+  lazymatch goal with
+  | |- reduce _ _ _ ?st1 _ _ _ ?st2 =>
+    let sta := fresh "st1" in
+    evar (sta : seq administrative_instruction);
+    let stb := fresh "st2" in
+    evar (stb : seq administrative_instruction);
+    let Est1 := fresh "E_before" in
+    assert (Est1: st1 = (l ++ sta) ++ r); [
+        rewrite/sta {sta stb}; try show_list_equality
+      | let Est2 := fresh "E_after" in
+        assert (Est2: st2 = (l ++ stb) ++ r); [
+            rewrite/stb {Est1 sta stb}; try show_list_equality
+          | rewrite Est1 Est2;
+            apply r_elimr with (les := r);
+            apply r_eliml with (lconst := l); first try solve_const_list;
+            rewrite /sta /stb {Est1 Est2 sta stb};
+            try by repeat constructor ] ]
+  end.
+
+(** Same as [frame_out], by the frames are inferred (syntactically). **)
+Ltac auto_frame :=
+  simplify_lists;
+  let empty := constr:([::] : list administrative_instruction) in
+  let left _ :=
+    repeat rewrite -catA;
+    repeat lazymatch goal with
+    | |- reduce _ _ _ (?l ++ _) _ _ _ (?l ++ _) =>
+      frame_out l empty
+    | |- reduce _ _ _ (?l ++ _) _ _ _ ?l =>
+      frame_out l empty
+    | |- reduce _ _ _ ?l _ _ _ (?l ++ _) =>
+      frame_out l empty
+    end in
+  let right _ :=
+    repeat rewrite catA;
+    repeat lazymatch goal with
+    | |- reduce _ _ _ (_ ++ ?r) _ _ _ (_ ++ ?r) =>
+      frame_out empty r
+    | |- reduce _ _ _ (_ ++ ?r) _ _ _ ?r =>
+      frame_out empty r
+    | |- reduce _ _ _ ?r _ _ _ (_ ++ ?r) =>
+      frame_out empty r
+    end;
+    (** Renormalising back. **)
+    repeat (rewrite -catA) in
+  repeat first [ progress left tt | progress right tt ].
+
+(** Same as [frame_out], by the frames are existential variables. **)
+Ltac eframe :=
+  let l := fresh "l" in
+  evar (l : seq administrative_instruction);
+  let r := fresh "r" in
+  evar (r : seq administrative_instruction);
+  frame_out l r.
+
+(***********)
+
+From Wasm Require Import interpreter_func_sound.
+
 (* rt: rt_step, rt_refl, rt_trans *)
-(* From CertiCoq Require Import CodegenWASM.LamdaANF_to_WASM. *)
 Check instance.
 Print instance.
 Lemma test_reduces (inst : instance) (hs_initial : host_state)
                    (hs_result : host_state) :
-  reduce_trans (hs_initial, empty_store_record host_function, Build_frame [] inst , map AI_basic (* test_function.(modfunc_body) *) [BI_const (nat_to_i32 1); BI_const (nat_to_i32 3); BI_binop T_i32 (Binop_i BOI_add)] )
-               (hs_initial, empty_store_record host_function, Build_frame [] inst, [AI_basic (BI_const (nat_to_i32 4))]).
+  reduce_trans (hs_initial, empty_store_record host_function, Build_frame [nat_to_i32 1; nat_to_i32 2] inst , map AI_basic test_function.(modfunc_body) (* [BI_const (nat_to_i32 1); BI_const (nat_to_i32 3); BI_binop T_i32 (Binop_i BOI_add)] *) )
+               (hs_initial, empty_store_record host_function, Build_frame [nat_to_i32 1; nat_to_i32 2] inst, [AI_basic (BI_const (nat_to_i32 3))]).
 Proof.
-  apply rt_step. cbn. constructor. constructor. reflexivity.
+  cbn.
+  eapply rt_trans with (y := (?[hs], ?[sr], ?[f], ?[s] ++ ?[t])).
+  apply rt_step. cbn.
+  explode_and_simplify.
+  replace ([:: AI_basic (BI_get_local 0); AI_basic (BI_get_local 1);
+      AI_basic (BI_binop T_i32 (Binop_i BOI_add))]) with
+      ([:: AI_basic (BI_get_local 0)] ++ ([AI_basic (BI_get_local 1);
+      AI_basic (BI_binop T_i32 (Binop_i BOI_add))])).
+  - apply r_elimr. apply r_get_local. cbn. reflexivity.
+  - reflexivity.
+  - cbn.
+  eapply rt_trans with (y := (?[hs], ?[sr], ?[f], ?[s] ++ ?[t])).
+  eapply rt_step. cbn.
+  explode_and_simplify.
+  rewrite catA.
+  apply r_elimr.
+  - apply r_eliml; auto.
+  - apply r_get_local. reflexivity.
+  - cbn. apply rt_step. cbn. apply r_simple. constructor. cbn. reflexivity.
 Qed.
-
-
 End OpsemTest.
 
 From Wasm Require Import interpreter_func common operations opsem interpreter_func properties.
@@ -167,6 +700,54 @@ Qed.
 End InterpTest.
 
 (*
+Section OpsemTest.
+(* preamble pasted from interpreter_func_sound.v*)
+
+Variable host_function : eqType.
+Let store_record := store_record host_function.
+Let function_closure := function_closure host_function.
+(*Let administrative_instruction := administrative_instruction host_function.
+
+Let to_e_list : seq basic_instruction -> seq administrative_instruction := @to_e_list _.
+Let to_b_list : seq administrative_instruction -> seq basic_instruction := @to_b_list _.*)
+Let e_typing : store_record -> t_context -> seq administrative_instruction -> function_type -> Prop :=
+  @e_typing _.
+Let inst_typing : store_record -> instance -> t_context -> bool := @inst_typing _.
+
+Let host := host host_function.
+
+(*Let run_one_step_fuel := @run_one_step_fuel host_function.*)
+
+Let RS_crash := interpreter_func.RS_crash.
+Let RS_break := interpreter_func.RS_break.
+Let RS_return := interpreter_func.RS_return.
+Let RS_normal := interpreter_func.RS_normal.
+
+Variable host_instance : host.
+
+Let run_step_fuel := @run_step_fuel host_function host_instance.
+
+Let host_state := host_state host_instance.
+
+Let reduce : host_state -> store_record -> frame -> seq administrative_instruction ->
+             host_state -> store_record -> frame -> seq administrative_instruction -> Prop
+  := @reduce _ _.
+
+Variable host_application_impl : host_state -> store_record -> function_type -> host_function -> seq value ->
+                       (host_state * option (store_record * result)).
+
+Hypothesis host_application_impl_correct :
+  (forall hs s ft hf vs hs' hres, (host_application_impl hs s ft hf vs = (hs', hres)) -> host_application hs s ft hf vs hs' hres).
+
+
+Let run_one_step := @run_one_step host_function host_instance host_application_impl.
+Let run_step := @run_step host_function host_instance host_application_impl.
+Let run_step_with_fuel := @run_step_with_fuel host_function host_instance host_application_impl.
+Let run_v := @run_v host_function host_instance host_application_impl.
+
+
+Let executable_host := executable_host host_function.
+
 Import Monads.
 Import MonadNotation.
 
@@ -174,8 +755,12 @@ From Coq Require Import String.
 From Wasm Require Import interpreter.
 From mathcomp Require Import seq.
 
+Import TestModule.
+
+Unset Universe Checking.
 
 Check lookup_exported_function.
+
 Check name.
 Print name.
 
@@ -184,9 +769,9 @@ Check eqtype.Equality.type.
 Print interp_instantiate_wrapper.
 Definition to_seq {A} (l : list A) : seq A := l.
 
-Definition run : option nat :=
-  module <- test_module ;;
-  instantiated_module <- interp_instantiate_wrapper module ;;
+Definition run :=
+  interp_instantiate_wrapper host_function test_module.
+  Some instantiated_module.
   (* cfg_tuple <- lookup_exported_function (to_seq (list_byte_of_string "add_i32")) instantiated_module;;*)
   Some 1.
 *)
